prove the entire BmapAlloc

src/BmapAllocMod.v
@@ -29,17 +29,17 @@ Definition freebit (bm:State) (off:BlocksPartDisk.addr) :=
 
 Inductive step {R:Type} : @progstate R Prog State ->
                           @progstate R Prog State -> Prop :=
-  | StepAllocOK: forall d off rx,
-    highest (freebit d) off ->
+  | StepAllocOK: forall d n rx,
+    highest (freebit d) n ->
     step (PS (Alloc rx) d)
-         (PS (rx (Some off)) (setidx BlocksPartDisk.eq_addr_dec d off InUse))
+         (PS (rx (Some n)) (setidx BlocksPartDisk.eq_addr_dec d n InUse))
   | StepAllocOut: forall d rx,
-    (~exists off, freebit d off) ->
+    (~exists n, freebit d n) ->
     step (PS (Alloc rx) d)
          (PS (rx None) d)
-  | StepFree: forall d off rx,
-    step (PS (Free off rx) d)
-         (PS (rx tt) (setidx BlocksPartDisk.eq_addr_dec d off Avail)).
+  | StepFree: forall d n rx,
+    step (PS (Free n rx) d)
+         (PS (rx tt) (setidx BlocksPartDisk.eq_addr_dec d n Avail)).
 Definition Step := @step.
 
 End BmapAlloc.
@@ -53,11 +53,73 @@ Program Definition pair2addr (bn:blockmapnum) (off:blockmapoff) : BlocksPartDisk
   bn * SizeBlock + off.
 Solve Obligations using Tactics.program_simpl; omega'.
 
-Program Definition addr2pair (n:BlocksPartDisk.addr) : blockmapnum * blockmapoff :=
-  (n / SizeBlock, n mod SizeBlock).
-Solve Obligations using intros; apply Nat.div_lt_upper_bound || apply Nat.mod_upper_bound; omega'.
+Program Definition addr2bn (n:BlocksPartDisk.addr) : blockmapnum :=
+  n / SizeBlock.
+Solve Obligations using intros; apply Nat.div_lt_upper_bound; omega'.
 
-Program Fixpoint Compile {R:Type} (p:BmapAlloc.Prog R) : BmapAllocPair.Prog R :=
+Program Definition addr2off (n:BlocksPartDisk.addr) : blockmapoff :=
+  n mod SizeBlock.
+Solve Obligations using intros; apply Nat.mod_upper_bound; omega'.
+
+Opaque modulo div.
+Lemma eq_bnoff_dec:
+  forall a b,
+  {a=b} +
+  {a<>b /\ addr2bn a<>addr2bn b} +
+  {a<>b /\ addr2bn a=addr2bn b /\ addr2off a <> addr2off b}.
+Proof.
+  intros.
+  destruct (eq_nat_dec (proj1_sig a) (proj1_sig b)) as [|Hab];
+    [ left; left; apply sig_pi; crush | ].
+  destruct (eq_nat_dec (proj1_sig (addr2bn a)) (proj1_sig (addr2bn b))) as [HBab|];
+    [ | left; right; split; apply sig_pi_ne; auto ].
+  right; split; [ apply sig_pi_ne; crush | ].
+  split; [ apply sig_pi; crush | ].
+  unfold not in *; intro HOab; apply Hab; clear Hab.
+  destruct a as [a]; destruct b as [b].
+  unfold addr2off in *; unfold addr2bn in *; unfold proj1_sig in *.
+  inversion HOab as [HOab']; clear HOab.
+  rewrite (Nat.div_mod a SizeBlock); [|omega'].
+  rewrite HBab. rewrite HOab'.
+  rewrite <- (Nat.div_mod b SizeBlock); [|omega'].
+  reflexivity.
+Qed.
+
+Lemma addr2pair2addr:
+  forall n,
+  pair2addr (addr2bn n) (addr2off n) = n.
+Proof.
+  intros; unfold addr2bn; unfold addr2off; unfold pair2addr; apply sig_pi; simpl.
+  rewrite Mult.mult_comm.
+  rewrite <- Nat.div_mod; omega'.
+Qed.
+Hint Rewrite addr2pair2addr.
+
+Lemma pair2addr2bn:
+  forall bn off,
+  addr2bn (pair2addr bn off) = bn.
+Proof.
+  intros; unfold addr2bn; unfold pair2addr; apply sig_pi; simpl.
+  rewrite Nat.div_add_l; [|omega'].
+  rewrite Nat.div_small; omega'.
+Qed.
+Hint Rewrite pair2addr2bn.
+
+Lemma pair2addr2off:
+  forall bn off,
+  addr2off (pair2addr bn off) = off.
+Proof.
+  intros; unfold addr2bn; unfold pair2addr; apply sig_pi; simpl.
+  rewrite Plus.plus_comm.
+  rewrite Nat.mod_add; [|omega'].
+  rewrite Nat.mod_small; omega'.
+Qed.
+Hint Rewrite pair2addr2off.
+Ltac rewrite_bn_off := repeat rewrite addr2pair2addr in *;
+                       repeat rewrite pair2addr2bn in *;
+                       repeat rewrite pair2addr2off in *.
+
+Fixpoint Compile {R:Type} (p:BmapAlloc.Prog R) : BmapAllocPair.Prog R :=
   match p with
   | BmapAlloc.Alloc rx =>
     x <- BmapAllocPair.Alloc;
@@ -66,8 +128,7 @@ Program Fixpoint Compile {R:Type} (p:BmapAlloc.Prog R) : BmapAllocPair.Prog R :=
     | Some (bn,off) => Compile (rx (Some (pair2addr bn off)))
     end
   | BmapAlloc.Free n rx =>
-    let (bn, off) := addr2pair n in
-    BmapAllocPair.Free bn off ;; Compile (rx tt)
+    BmapAllocPair.Free (addr2bn n) (addr2off n) ;; Compile (rx tt)
   | BmapAlloc.Return r =>
     BmapAllocPair.Return r
   end.
@@ -79,6 +140,42 @@ Inductive statematch : BmapAlloc.State -> BmapAllocPair.State -> Prop :=
 Definition StateMatch := statematch.
 Hint Constructors statematch.
 
+Ltac auto_omega' := auto; omega'.
+
+Lemma highest_bn:
+  forall fs s n,
+  statematch fs s ->
+  highest (BmapAlloc.freebit fs) n ->
+  highest (fun bn => exists off, BmapAllocOne.freebit (s bn) off) (addr2bn n).
+Proof.
+  unfold BmapAllocOne.freebit; unfold BmapAlloc.freebit; intros.
+  invert_rel (@highest (fun x => x < BlocksPartSize.Size)).
+  invert_rel statematch; subst.
+  split; [ exists (addr2off n); rewrite <- M; rewrite_bn_off; auto | ].
+  unfold not; intros; apply H2; clear H2.
+  destruct H as [bn H]. destruct H as [Hbn H]. destruct H as [off Havail].
+  exists (pair2addr bn off); split.
+  - rewrite <- (addr2pair2addr n). unfold pair2addr. omega'.
+  - crush.
+Qed.
+
+Lemma highest_off:
+  forall fs s n,
+  statematch fs s ->
+  highest (BmapAlloc.freebit fs) n ->
+  highest (BmapAllocOne.freebit (s (addr2bn n))) (addr2off n).
+Proof.
+  unfold BmapAllocOne.freebit; unfold BmapAlloc.freebit; intros.
+  invert_rel (@highest (fun x => x < BlocksPartSize.Size)).
+  invert_rel statematch; subst.
+  split; [ rewrite <- M; rewrite_bn_off; auto | ].
+  unfold not; intros; apply H2; clear H2.
+  destruct H as [off H]. destruct H as [Hoff Havail].
+  exists (pair2addr (addr2bn n) off); split.
+  - rewrite <- (addr2pair2addr n). rewrite pair2addr2bn. unfold pair2addr. omega'.
+  - crush.
+Qed.
+
 Theorem FSim:
   forall R,
   forward_simulation (BmapAlloc.Step R) (BmapAllocPair.Step R).
@@ -86,13 +183,34 @@ Proof.
   intros; fsim_begin (@Compile R) statematch.
 
   - (* Alloc Some *)
-    admit.
+    eexists; split.
+    + eapply star_step; [apply BmapAllocPair.StepAllocOK|].
+      * eapply highest_bn; eauto.
+      * eapply highest_off; eauto.
+      * fold (@Compile R).
+        apply star_refl.
+    + constructor; rewrite_bn_off; [auto|constructor]; intros.
+      destruct (eq_bnoff_dec n (pair2addr bn off)) as [H'|]; [destruct H'|];
+      Tactics.destruct_pairs;
+      subst; rewrite_bn_off; repeat resolve_setidx auto_omega'; auto.
 
   - (* Alloc None *)
-    admit.
+    eexists; split.
+    + eapply star_step; [apply BmapAllocPair.StepAllocOut|apply star_refl].
+      unfold not; intros. apply H3; clear H3.
+      unfold BmapAllocOne.freebit in *.
+      unfold BmapAlloc.freebit in *.
+      destruct H. destruct H.
+      eexists. rewrite M0. eauto.
+    + crush.
 
   - (* Free *)
-    admit.
+    eexists; split.
+    + eapply star_step; [constructor|apply star_refl].
+    + constructor; [auto|constructor]; intros.
+      destruct (eq_bnoff_dec n (pair2addr bn off)) as [H'|]; [destruct H'|];
+      Tactics.destruct_pairs;
+      subst; rewrite_bn_off; repeat resolve_setidx auto_omega'; auto.
 Qed.
 
 End BmapAllocToAllocPair.
